Pattern matching is now in the option monad instead of micro.

rocq-osiris/theories/program_logic/pure/pattern_rules.v
@@ -1,7 +1,6 @@
 From osiris Require Import base.
 From osiris.lang Require Import syntax encode notations locations.
 From osiris.semantics Require Import semantics.
-From osiris.program_logic.pure Require Import pure_rules.
 
 Open Scope Z_scope.
 
@@ -17,85 +16,99 @@ Open Scope Z_scope.
    results in an extended environment that satisfies [φ]
    or fails (by reducing to [throw ()]) and guarantees [ψ]. *)
 
-Definition cpattern η δ p o (φ : env -> Prop) (ψ : Prop) :=
-  pure_wp (eval_cpat η δ p o) φ (λ (_ : unit), ψ).
+Definition cpattern η δ p o (φ : env -> Prop) (ζ : Prop) :=
+  match eval_cpat η δ p o with
+  | Some η => φ η
+  | None => ζ
+  end.
 
-Definition pattern η δ p v (φ : env -> Prop) (ψ : Prop) :=
-  pure_wp (eval_pat η δ p v) φ (λ (_ : unit), ψ).
+Definition pattern η δ p v (φ : env -> Prop) (ζ : Prop) :=
+  match eval_pat η δ p v with
+  | Some η => φ η
+  | None => ζ
+  end.
 
-Definition patterns η δ ps vs (φ : env -> Prop) (ψ : Prop) :=
-  pure_wp (eval_pats η δ ps vs) φ (λ (_ : unit), ψ).
+Definition patterns η δ ps vs (φ : env -> Prop) (ζ : Prop) :=
+  match eval_pats η δ ps vs with
+  | Some η => φ η
+  | None => ζ
+  end.
+
+Lemma union_None_l {A} (o : option A) :
+  None ∪ o = o.
+Proof. by destruct o. Qed.
 
 (* -------------------------------------------------------------------------- *)
 
 Section pattern_rules.
 
   Implicit Type φ : env -> Prop.
-  Implicit Type ψ : Prop.
+  Implicit Type ζ : Prop.
 
   (* Monotonicity properties for [cpattern], [pattern], and [patterns]. *)
 
-  Lemma cpattern_mono η δ p v (φ φ' : env -> Prop) (ψ ψ' : Prop) :
-    cpattern η δ p v φ ψ →
+  Lemma cpattern_mono η δ p v (φ φ' : env -> Prop) (ζ ζ' : Prop) :
+    cpattern η δ p v φ ζ →
     (∀ δ, φ δ → φ' δ) →
-    (ψ → ψ') →
-    cpattern η δ p v φ' ψ'.
+    (ζ → ζ') →
+    cpattern η δ p v φ' ζ'.
   Proof.
-    unfold cpattern; eauto using pure_wp_mono.
+    unfold cpattern.
+    destruct (eval_cpat η δ p v); auto.
   Qed.
 
-  Lemma cpattern_env_mono η δ p v (φ φ' : env -> Prop) (ψ : Prop) :
-    cpattern η δ p v φ ψ →
+  Lemma cpattern_env_mono η δ p v (φ φ' : env -> Prop) (ζ : Prop) :
+    cpattern η δ p v φ ζ →
     (∀ δ, φ δ → φ' δ) →
-    cpattern η δ p v φ' ψ.
+    cpattern η δ p v φ' ζ.
   Proof. intros; by eapply cpattern_mono. Qed.
 
-  Lemma cpattern_exn_mono η δ p v (φ : env -> Prop) (ψ ψ': Prop) :
-    cpattern η δ p v φ ψ →
-    (ψ → ψ') →
-    cpattern η δ p v φ ψ'.
+  Lemma cpattern_mono_exn η δ p v (φ : env -> Prop) (ζ ζ': Prop) :
+    cpattern η δ p v φ ζ →
+    (ζ → ζ') →
+    cpattern η δ p v φ ζ'.
   Proof. intros; by eapply cpattern_mono. Qed.
 
-  Lemma pattern_mono η δ p v (φ φ' : env -> Prop) (ψ ψ' : Prop) :
-    pattern η δ p v φ ψ →
+  Lemma pattern_mono η δ p v (φ φ' : env -> Prop) (ζ ζ' : Prop) :
+    pattern η δ p v φ ζ →
     (∀ δ, φ δ → φ' δ) →
-    (ψ → ψ') →
-    pattern η δ p v φ' ψ'.
+    (ζ → ζ') →
+    pattern η δ p v φ' ζ'.
   Proof.
-    unfold pattern; eauto using pure_wp_mono.
+    unfold pattern. destruct (eval_pat η δ p v); auto.
   Qed.
 
-  Lemma pattern_env_mono η δ p v (φ φ' : env -> Prop) (ψ : Prop) :
-    pattern η δ p v φ ψ →
+  Lemma pattern_env_mono η δ p v (φ φ' : env -> Prop) (ζ : Prop) :
+    pattern η δ p v φ ζ →
     (∀ δ, φ δ → φ' δ) →
-    pattern η δ p v φ' ψ.
+    pattern η δ p v φ' ζ.
   Proof. intros; by eapply pattern_mono. Qed.
 
-  Lemma pattern_exn_mono η δ p v (φ : env -> Prop) (ψ ψ': Prop) :
-    pattern η δ p v φ ψ →
-    (ψ → ψ') →
-    pattern η δ p v φ ψ'.
+  Lemma pattern_mono_exn η δ p v (φ : env -> Prop) (ζ ζ': Prop) :
+    pattern η δ p v φ ζ →
+    (ζ → ζ') →
+    pattern η δ p v φ ζ'.
   Proof. intros; by eapply pattern_mono. Qed.
 
-  Lemma patterns_mono η δ ps vs (φ φ' : env -> Prop) (ψ ψ' : Prop) :
-    patterns η δ ps vs φ ψ →
+  Lemma patterns_mono η δ ps vs (φ φ' : env -> Prop) (ζ ζ' : Prop) :
+    patterns η δ ps vs φ ζ →
     (∀ η, φ η → φ' η) →
-    (ψ → ψ') →
-    patterns η δ ps vs φ' ψ'.
+    (ζ → ζ') →
+    patterns η δ ps vs φ' ζ'.
   Proof.
-    unfold patterns; eauto using pure_wp_mono.
+    unfold patterns; destruct (eval_pats η δ ps vs); auto.
   Qed.
 
-  Lemma patterns_env_mono η δ ps vs (φ φ' : env -> Prop) (ψ : Prop) :
-    patterns η δ ps vs φ ψ →
+  Lemma patterns_env_mono η δ ps vs (φ φ' : env -> Prop) (ζ : Prop) :
+    patterns η δ ps vs φ ζ →
     (∀ δ, φ δ → φ' δ) →
-    patterns η δ ps vs φ' ψ.
+    patterns η δ ps vs φ' ζ.
   Proof. intros; by eapply patterns_mono. Qed.
 
-  Lemma patterns_exn_mono η δ ps vs (φ : env -> Prop) (ψ ψ': Prop) :
-    patterns η δ ps vs φ ψ →
-    (ψ → ψ') →
-    patterns η δ ps vs φ ψ'.
+  Lemma patterns_mono_exn η δ ps vs (φ : env -> Prop) (ζ ζ': Prop) :
+    patterns η δ ps vs φ ζ →
+    (ζ → ζ') →
+    patterns η δ ps vs φ ζ'.
   Proof. intros; by eapply patterns_mono. Qed.
 
   (* -------------------------------------------------------------------------- *)
@@ -108,14 +121,14 @@ Section pattern_rules.
     negative formula. The positive formula, the postcondition [φ],
     accumulates a sequence of universal quantifiers and equations that
     describe what is learnt when pattern matching succeeds. The negative
-    formula, the failure postcondition [ψ], describes what is learnt when
+    formula, the failure postcondition [ζ], describes what is learnt when
     pattern matching fails. *)
 
   (* When a pattern cannot fail or can fail due to several distinct causes,
     a naive statement of its reasoning rule would have one occurrence of
-    [ψ] in its conclusion and no occurrence or multiple occurrences of [ψ]
+    [ζ] in its conclusion and no occurrence or multiple occurrences of [ζ]
     in its premises. From an operational point of view, this is
-    undesirable, because [ψ] is then unconstrained or duplicated. We avoid
+    undesirable, because [ζ] is then unconstrained or duplicated. We avoid
     this phenomenon by using [False] or a disjunction in the conclusion of
     the reasoning rule. Thus, from an operational point of view, applying
     the reasoning rule instantiates the failure postcondition with a
@@ -125,14 +138,14 @@ Section pattern_rules.
     φ δ →
     pattern η δ PAny v φ False.
   Proof.
-    unfold pattern. simpl_eval_pat. eauto using pure_wp_ret.
+    unfold pattern. simpl_eval_pat. auto.
   Qed.
 
   Lemma pat_PVar η δ x v φ :
     φ ((x, v) :: δ) →
     pattern η δ (PVar x) v φ False.
   Proof.
-    unfold pattern. simpl_eval_pat. eauto using pure_wp_ret.
+    unfold pattern. simpl_eval_pat. auto.
   Qed.
 
   (* Given a goal of the form [pattern η (PVar x) v ?φ False],
@@ -151,24 +164,25 @@ Section pattern_rules.
         (apply pat_PVar2 || eapply pat_PVar)
     end.
 
-  Lemma pat_PAlias η δ p x v φ ψ :
-    pattern η δ p v (λ δ, φ ((x, v) :: δ)) ψ →
-    pattern η δ (PAlias p x) v φ ψ.
+  Lemma pat_PAlias η δ p x v φ ζ :
+    pattern η δ p v (λ δ, φ ((x, v) :: δ)) ζ →
+    pattern η δ (PAlias p x) v φ ζ.
   Proof.
     unfold pattern. simpl_eval_pat; intros.
-    apply pure_wp_bind.
-    eauto using pure_wp_mono, pure_wp_ret.
+    destruct (eval_pat η δ p v); auto.
   Qed.
 
-  Lemma pat_POr η δ p1 p2 v φ ψ1 ψ2 :
-    pattern η δ p1 v φ ψ1 →
-    (ψ1 → pattern η δ p2 v φ ψ2) →
-    pattern η δ (POr p1 p2) v φ (ψ1 ∧ ψ2).
-      (* The conjunction [ψ1 ∧ ψ2] reflects the fact that, for the
+  Lemma pat_POr η δ p1 p2 v φ ζ1 ζ2 :
+    pattern η δ p1 v φ ζ1 →
+    (ζ1 → pattern η δ p2 v φ ζ2) →
+    pattern η δ (POr p1 p2) v φ (ζ1 ∧ ζ2).
+      (* The conjunction [ζ1 ∧ ζ2] reflects the fact that, for the
         disjunction pattern to fail, both sides must fail. *)
   Proof.
     unfold pattern. simpl_eval_pat; intros.
-    eauto using pure_wp_orelse, pure_wp_mono.
+    destruct (eval_pat η δ p1 v).
+    - by rewrite union_Some_l.
+    - destruct (eval_pat η δ p2 v); simpl; auto.
   Qed.
 
   Lemma pat_PUnit η δ v φ :
@@ -176,69 +190,66 @@ Section pattern_rules.
     v = #() →
     pattern η δ PUnit v φ False.
   Proof.
-    unfold pattern. intros ? ->; simpl_eval_pat.
-    eauto using pure_wp_ret.
+    unfold pattern. intros ? ->; simpl_eval_pat; auto.
   Qed.
 
-  Lemma pat_PTuple `{Encode A} η δ ps (a : A) vs φ ψ :
+  Lemma pat_PTuple `{Encode A} η δ ps (a : A) vs φ ζ :
     #a = VTuple vs ->
-    patterns η δ ps vs φ ψ →
-    pattern η δ (PTuple ps) #a φ ψ.
+    patterns η δ ps vs φ ζ →
+    pattern η δ (PTuple ps) #a φ ζ.
   Proof.
     unfold patterns, pattern.
     intros ->. by simpl_eval_pat.
   Qed.
 
-  Lemma pat_PTuple_val δ η ps vs φ ψ :
-    patterns δ η ps vs φ ψ ->
-    pattern δ η (PTuple ps) (VTuple vs) φ ψ.
+  Lemma pat_PTuple_val δ η ps vs φ ζ :
+    patterns δ η ps vs φ ζ ->
+    pattern δ η (PTuple ps) (VTuple vs) φ ζ.
   Proof.
     unfold pattern. by simpl_eval_pat.
   Qed.
 
-  Lemma pat_PPair `{Encode A, Encode B} η δ p1 p2 v1 v2 (x1 : A) (x2 : B) φ ψ1 ψ2 :
+  Lemma pat_PPair `{Encode A, Encode B} η δ p1 p2 v1 v2 (x1 : A) (x2 : B) φ ζ1 ζ2 :
     v1 = #x1 ->
     v2 = #x2 ->
-    pattern η δ p1 #x1 (λ δ', pattern η δ' p2 #x2 φ (ψ2)) (ψ1) ->
-    pattern η δ (PPair p1 p2) (VPair v1 v2) φ (ψ1 \/ ψ2).
+    pattern η δ p1 #x1 (λ δ', pattern η δ' p2 #x2 φ (ζ2)) (ζ1) ->
+    pattern η δ (PPair p1 p2) (VPair v1 v2) φ (ζ1 \/ ζ2).
   Proof.
     intros; subst.
-    unfold pattern. simpl_eval_pat.
-    eapply pure_wp_bind_conseq; [ eapply pure_wp_mono; eauto | ].
-    simpl; intros. rewrite bind_ret_right.
-    eapply pure_wp_bind_conseq; [ eapply pure_wp_mono; eauto | ].
-    auto using pure_wp_ret.
+    unfold pattern in H3 |- *. simpl_eval_pat.
+    destruct (eval_pat η δ p1 #x1); simpl; last auto.
+    destruct (eval_pat η e p2 #x2); simpl; auto.
   Qed.
 
-  Lemma pat_PData_nil η δ c c' φ ψ :
+  Lemma pat_PData_nil η δ c c' φ ζ :
     (c = c' -> φ δ) ->
-    pattern η δ (PData c nil) (VData c' nil) φ (ψ ∨ c ≠ c').
+    pattern η δ (PData c nil) (VData c' nil) φ (ζ ∨ c ≠ c').
       (* This form is useful when the truth of the equality [c = c']
         is not statically known. *)
   Proof.
     unfold pattern; intros. simpl_eval_pat.
-    destruct_string_eqb;
-      eauto using pure_wp_throw, pure_mono, pure_wp_ret.
+    destruct_string_eqb; auto.
   Qed.
 
-  Lemma pat_PData_or η δ c c' ps vs φ ψ :
-    (c = c' -> patterns η δ ps vs φ ψ) ->
-    pattern η δ (PData c ps) (VData c' vs) φ (ψ ∨ c ≠ c').
+  Lemma pat_PData_or η δ c c' ps vs φ ζ :
+    (c = c' -> patterns η δ ps vs φ ζ) ->
+    pattern η δ (PData c ps) (VData c' vs) φ (ζ ∨ c ≠ c').
       (* This form is useful when the truth of the equality [c = c']
         is not statically known. *)
   Proof.
     unfold pattern; intros. simpl_eval_pat.
-    destruct_string_eqb; eauto using pure_wp_throw.
-    eapply pure_wp_mono; first apply H; eauto.
+    destruct_string_eqb; eauto.
+    eapply patterns_mono; first apply H; eauto.
   Qed.
 
-  Lemma pat_PData_eq η δ c ps vs φ ψ :
-    patterns η δ ps vs φ ψ →
-    pattern η δ (PData c ps) (VData c vs) φ ψ.
+  Lemma pat_PData_eq η δ c ps vs φ ζ :
+    patterns η δ ps vs φ ζ →
+    pattern η δ (PData c ps) (VData c vs) φ ζ.
       (* This form is useful when [c = c'] is statically known. *)
   Proof.
     unfold pattern; intros. simpl_eval_pat.
-    destruct_string_eqb; solve [ eauto using pure_wp_throw | tauto ].
+    destruct_string_eqb; eauto.
+    contradiction.
   Qed.
 
   Lemma pat_PData_neq η δ c ps c' vs φ :
@@ -247,7 +258,8 @@ Section pattern_rules.
       (* This form is useful when [c ≠ c'] is statically known. *)
   Proof.
     unfold pattern; intros. simpl_eval_pat.
-    destruct_string_eqb; solve [ eauto using pure_wp_throw | tauto ].
+    destruct_string_eqb; eauto.
+    contradiction.
   Qed.
 
   Lemma pat_PData η δ c ps c' v vs φ :
@@ -256,66 +268,49 @@ Section pattern_rules.
     pattern η δ (PData c ps) v φ True.
   Proof.
     unfold pattern; intros. simpl_eval_pat. subst.
-    destruct_string_eqb; solve [ eauto using pure_wp_throw | tauto ].
+    destruct_string_eqb; auto.
+    apply (H0 Heq).
   Qed.
 
   (* This more general version is not used in tactics at the moment *)
-  Lemma pat_PXData η δ π ps l l' vs φ ψ :
-    lookup_path η π = ret (VLoc l') →
-    (l = l' → patterns η δ ps vs φ ψ) →
-    pattern η δ (PXData π ps) (VXData l vs) φ (ψ ∨ l ≠ l').
+  Lemma pat_PXData η δ π ps l l' vs φ ζ :
+    lookup_path η π = Some #l' →
+    (l = l' → patterns η δ ps vs φ ζ) →
+    pattern η δ (PXData π ps) (VXData l vs) φ (ζ ∨ l ≠ l').
   Proof.
     unfold pattern. simpl_eval_pat. intros ->.
-    change (as_loc (widen (ret (VLoc l')))) with (@ret _ unit l').
-    rewrite bind_ret.
+    simpl.
     destruct (eqb_spec l l').
-    - firstorder eauto using pure_wp_mono_throw.
-    - rewrite <-pure_wp_reversible_throw. auto.
+    - intros. eapply patterns_mono_exn; eauto.
+    - tauto.
   Qed.
 
-  Lemma pat_PXData_eq η δ π ps l vs φ ψ :
-    lookup_path η π = ret (VLoc l) ->
-    patterns η δ ps vs φ ψ →
-    pattern η δ (PXData π ps) (VXData l vs) φ ψ.
+  Lemma pat_PXData_eq η δ π ps l vs φ ζ :
+    lookup_path η π = Some #l ->
+    patterns η δ ps vs φ ζ →
+    pattern η δ (PXData π ps) (VXData l vs) φ ζ.
       (* This form is useful when the truth of the equality [c = c']
         is not statically known. *)
   Proof.
     unfold pattern; intros Hlookup Hpat.
-    simpl_eval_pat; rewrite Hlookup. cbn; rewrite bind_ret.
+    simpl_eval_pat; rewrite Hlookup. simpl.
     unfold locations.eqb; destruct l; cbn.
     by rewrite Z.eqb_refl.
   Qed.
 
   Lemma pat_PXData_neq η δ π ps l1 l2 vs φ :
-    lookup_path η π = ret (VLoc l1) ->
+    lookup_path η π = Some #l1 ->
     (address l1 <> address l2) ->
     pattern η δ (PXData π ps) (VXData l2 vs) φ True.
       (* This form is useful when the truth of the equality [c = c']
         is not statically known. *)
   Proof.
     unfold pattern; intros Hlookup Heq; simpl_eval_pat.
-    rewrite Hlookup. cbn; rewrite bind_ret.
+    rewrite Hlookup. cbn.
     unfold locations.eqb; simpl.
     destruct l1, l2; simpl in *.
-    replace (address0 =? address) with false;
-      last by apply eq_sym; apply Z.eqb_neq.
-    by apply pure_wp_throw.
-  Qed.
-
-  Lemma pat_PXData_neq' η δ π ps l1 l2 vs :
-    lookup_path η π = ret (VLoc l1) ->
-    (address l1 <> address l2) ->
-    pattern η δ (PXData π ps) (VXData l2 vs) (λ _, False) True.
-      (* This form is useful when the truth of the equality [c = c']
-        is not statically known. *)
-  Proof.
-    unfold pattern; intros Hlookup Heq; simpl_eval_pat.
-    rewrite Hlookup. cbn; rewrite bind_ret.
-    unfold locations.eqb; simpl.
-    destruct l1, l2; simpl in *.
-    replace (address0 =? address) with false;
-      last by apply eq_sym; apply Z.eqb_neq.
-    by apply pure_wp_throw.
+    apply Z.eqb_neq in Heq.
+    by rewrite Z.eqb_sym, Heq.
   Qed.
 
   (* -------------------------------------------------------------------------- *)
@@ -326,39 +321,33 @@ Section pattern_rules.
     φ δ →
     patterns η δ [] [] φ False.
   Proof.
-    unfold patterns.
-    simpl_eval_pats.
-    eauto using pure_wp_ret.
+    unfold patterns. simpl_eval_pats. auto.
   Qed.
 
-  Lemma pats_PCons_unary η δ p ps v vs φ ψ1 ψ2 :
-    pattern η δ p v (λ δ, patterns η δ ps vs φ ψ2) ψ1 →
-    patterns η δ (p :: ps) (v :: vs) φ (ψ1 \/ ψ2).
+  Lemma pats_PCons_unary η δ p ps v vs φ ζ1 ζ2 :
+    pattern η δ p v (λ δ, patterns η δ ps vs φ ζ2) ζ1 →
+    patterns η δ (p :: ps) (v :: vs) φ (ζ1 \/ ζ2).
   Proof.
-    unfold patterns, patterns. intros Hp; simpl_eval_pats.
-    eapply pure_wp_bind_conseq.
-    { eapply pure_wp_mono.
-      - eassumption.
-      - simpl; intros. eapply pure_wp_mono; eauto.
-      - tauto. }
-    simpl; intros. rewrite bind_ret_right.
-    eapply pure_wp_mono; eauto.
+    unfold patterns, pattern. intros Hp; simpl_eval_pats.
+    destruct (eval_pat η δ p v); simpl.
+    - rewrite bind_with_Some.
+      eapply patterns_mono_exn; eauto.
+    - tauto.
   Qed.
 
   Lemma pats_PCons_unary_false η δ p ps v vs φ :
     pattern η δ p v (λ δ, patterns η δ ps vs φ False) False ->
     patterns η δ (p :: ps) (v :: vs) φ False.
   Proof.
-    intros.
-    assert (False \/ False -> False) as HFalse by tauto.
-    eapply patterns_exn_mono; [ clear HFalse | exact HFalse ].
-    by apply pats_PCons_unary.
+    intros. eapply patterns_mono_exn.
+    { apply pats_PCons_unary, H. }
+    tauto.
   Qed.
 
-  Lemma pats_PCons η δ p ps v vs φ' φ ψ1 ψ2 :
-    pattern η δ p v φ' ψ1 →
-    (∀ δ, φ' δ → patterns η δ ps vs φ ψ2) →
-    patterns η δ (p :: ps) (v :: vs) φ (ψ1 ∨ ψ2).
+  Lemma pats_PCons η δ p ps v vs φ' φ ζ1 ζ2 :
+    pattern η δ p v φ' ζ1 →
+    (∀ δ, φ' δ → patterns η δ ps vs φ ζ2) →
+    patterns η δ (p :: ps) (v :: vs) φ (ζ1 ∨ ζ2).
   Proof.
     intros. eapply pats_PCons_unary.
     eapply pattern_mono; eauto.
@@ -392,18 +381,17 @@ Section pattern_rules.
     pattern η δ (PConstant c) (VConstant c) φ False.
   Proof.
     intros Hφ.
-    eapply pattern_exn_mono; [ eapply pat_PConst; eauto | tauto ].
+    eapply pattern_mono_exn; [ eapply pat_PConst; eauto | tauto ].
   Qed.
 
-  Lemma pat_PConst_neq η δ c c' e ψ :
+  Lemma pat_PConst_neq η δ c c' e ζ :
     c <> c' ->
-    ψ ->
-    pattern η δ (PConstant c) (VData c' e) (λ _, False) ψ.
+    ζ ->
+    pattern η δ (PConstant c) (VData c' e) (λ _, False) ζ.
   Proof.
-    intros Hneq Hψ.
+    intros Hneq Hζ.
     unfold pattern. simpl_eval_pat.
-    apply String.eqb_neq in Hneq as ->.
-    by apply pure_wp_throw.
+    by apply String.eqb_neq in Hneq as ->.
   Qed.
 
   Lemma pat_false η δ v (P : Prop) φ :
@@ -419,7 +407,7 @@ Section pattern_rules.
         [ by simpl | by apply truth_true_elim].
       done. }
 
-    { eapply pattern_exn_mono.
+    { eapply pattern_mono_exn.
       eapply pat_PConst_eq;
         auto using truth_false_elim.
       tauto. }
@@ -433,7 +421,7 @@ Section pattern_rules.
     intros -> Hφ; simpl.
     destruct (truth P) eqn:?.
 
-    { eapply pattern_exn_mono.
+    { eapply pattern_mono_exn.
       eapply pat_PConst_eq;
         apply Hφ; by apply truth_true_elim.
       tauto. }
@@ -455,44 +443,45 @@ Section pattern_rules.
     unfold pattern; simpl_eval_pat.
     rewrite int.eq_repr_repr; auto.
     destruct (_ =? _) eqn:E.
-    - apply pure_wp_ret. apply Hφ. by apply Z.eqb_eq.
-    - apply pure_wp_throw. by apply Z.eqb_neq.
+    - apply Hφ. by apply Z.eqb_eq.
+    - by apply Z.eqb_neq.
   Qed.
 
   (* -------------------------------------------------------------------------- *)
 
-  Lemma cpat_CVal η δ p v φ ψ :
-    pattern η δ p v φ ψ ->
-    cpattern η δ (CVal p) (O2Ret v) φ ψ.
+  Lemma cpat_CVal η δ p v φ ζ :
+    pattern η δ p v φ ζ ->
+    cpattern η δ (CVal p) (O2Ret v) φ ζ.
   Proof.
     tauto.
   Qed.
 
-  Lemma cpat_CExc η δ p v φ ψ :
-    pattern η δ p v φ ψ ->
-    cpattern η δ (CExc p) (O2Throw v) φ ψ.
+  Lemma cpat_CExc η δ p v φ ζ :
+    pattern η δ p v φ ζ ->
+    cpattern η δ (CExc p) (O2Throw v) φ ζ.
   Proof.
     tauto.
   Qed.
 
-  Lemma cpat_COr η δ cp1 cp2 o φ ψ1 ψ2 :
-    cpattern η δ cp1 o φ ψ1 ->
-    (ψ1 → cpattern η δ cp2 o φ ψ2) ->
-    cpattern η δ (COr cp1 cp2) o φ (ψ1 /\ ψ2).
+  Lemma cpat_COr η δ cp1 cp2 o φ ζ1 ζ2 :
+    cpattern η δ cp1 o φ ζ1 ->
+    (ζ1 → cpattern η δ cp2 o φ ζ2) ->
+    cpattern η δ (COr cp1 cp2) o φ (ζ1 /\ ζ2).
   Proof.
-    unfold cpattern. intros.
-    eapply pure_wp_orelse; [ eassumption | ].
-    eauto using pure_wp_mono.
+    unfold cpattern. intros. simpl eval_cpat.
+    destruct (eval_cpat η δ cp1 o).
+    - by rewrite union_Some_l.
+    - destruct (eval_cpat η δ cp2 o); simpl; tauto.
   Qed.
 
-  Lemma cpat_CEff η δ peff pk v k φ ψ1 ψ2 :
-    pattern η δ peff v (λ δ, pattern η δ pk (VCont k) φ ψ2) ψ1 ->
-    cpattern η δ (CEff peff pk) (O3Perform v k) φ (ψ1 \/ ψ2).
+  Lemma cpat_CEff η δ peff pk v k φ ζ1 ζ2 :
+    pattern η δ peff v (λ δ, pattern η δ pk (VCont k) φ ζ2) ζ1 ->
+    cpattern η δ (CEff peff pk) (O3Perform v k) φ (ζ1 \/ ζ2).
   Proof.
     unfold cpattern, pattern; intros. simpl.
-    eapply pure_wp_bind_conseq; [ eapply pure_wp_mono; eauto | ].
-    simpl.
-    eauto using pure_wp_mono.
+    destruct (eval_pat η δ peff v); simpl.
+    - eapply pattern_mono_exn; eauto.
+    - tauto.
   Qed.
 
   Fixpoint valid_cpattern_match {A E} cp (o : outcome3 A E) :=
@@ -509,26 +498,24 @@ Section pattern_rules.
 
   Lemma invert_valid_match cp o :
     valid_cpattern_match cp o = false ->
-    ∀ η δ, eval_cpat η δ cp o = throw ().
+    ∀ η δ, eval_cpat η δ cp o = None.
   Proof.
     intros Hvalid η δ.
     induction cp; destruct o; simpl in *; try congruence;
       (* Only the [COr cp1 cp2] case remains. *)
-      unfold orelse;
       apply orb_false_elim in Hvalid as [H1 H2];
       apply IHcp1 in H1; apply IHcp2 in H2;
-      by rewrite H1, H2, !try_throw.
+      apply union_None; auto.
   Qed.
 
-  Lemma cpat_mismatch η δ cp o φ (ψ : Prop) :
+  Lemma cpat_mismatch η δ cp o φ (ζ : Prop) :
     valid_cpattern_match cp o = false ->
-    ψ ->
-    cpattern η δ cp o φ ψ.
+    ζ ->
+    cpattern η δ cp o φ ζ.
   Proof.
     intros.
     unfold cpattern.
-    rewrite invert_valid_match by assumption.
-    by apply pure_wp_throw.
+    by rewrite invert_valid_match.
   Qed.
 
   (* -------------------------------------------------------------------------- *)
@@ -547,7 +534,7 @@ Section pattern_rules.
       with the knowledge that [xs] is not empty *)
   Proof.
     intros; subst.
-    destruct xs; eapply pattern_exn_mono.
+    destruct xs; eapply pattern_mono_exn.
     { eapply pat_PConst; eauto. }
     { tauto. }
     { eapply pat_PData_neq; done. }
@@ -559,19 +546,19 @@ Section pattern_rules.
     by evar instantiation scopes. *)
 
   Lemma pat_pCons_cut `{Encode A} v xs η δ p1 p2 φ (φ1 : A -> env -> Prop)
-    (ψ1 : A -> Prop) (ψ2 : list A -> Prop)
+    (ζ1 : A -> Prop) (ζ2 : list A -> Prop)
     :
     v = #xs ->
     (∀ (x : A) (xs' : list A),
         xs = x :: xs' →
-        pattern η δ p1 #x (φ1 x) (ψ1 x)) ->
+        pattern η δ p1 #x (φ1 x) (ζ1 x)) ->
         (* If [#x] matches [p1], we gain the knowledge [φ1 x η0].
-          Otherwise, we gain the knowledge [ψ1 x] *)
+          Otherwise, we gain the knowledge [ζ1 x] *)
     (∀ (x : A) (xs' : list A),
         xs = x :: xs' →
-        (forall δ', φ1 x δ' -> pattern η δ' p2 #xs' φ (ψ2 xs'))) ->
-        (* If [#xs'] does not match [p2], then we gain the knowledge [ψ2 xs'] *)
-    pattern η δ (pCons p1 p2) v φ (xs = [] \/ (exists x xs', xs = x :: xs' /\ (ψ1 x \/ ψ2 xs'))).
+        (forall δ', φ1 x δ' -> pattern η δ' p2 #xs' φ (ζ2 xs'))) ->
+        (* If [#xs'] does not match [p2], then we gain the knowledge [ζ2 xs'] *)
+    pattern η δ (pCons p1 p2) v φ (xs = [] \/ (exists x xs', xs = x :: xs' /\ (ζ1 x \/ ζ2 xs'))).
     (* There are three ways the match can be unsuccessful:
       - the list is empty
       - the list is non-empty, but its head did not match [p1]
@@ -579,29 +566,29 @@ Section pattern_rules.
   Proof.
     intros; subst.
     destruct xs.
-    { eapply pattern_exn_mono.
+    { eapply pattern_mono_exn.
       { by apply pat_PData_neq. }
       tauto. }
-    { eapply pattern_exn_mono.
+    { eapply pattern_mono_exn.
       { eapply pat_PData_eq; pats.  }
       right; do 2 eexists; split; [ reflexivity | tauto ]. }
   Qed.
 
   Lemma pat_pCons `{Encode A} v xs η δ p1 p2 φ
-    (ψ1 : A -> Prop) (ψ2 : list A -> Prop)
+    (ζ1 : A -> Prop) (ζ2 : list A -> Prop)
     :
     v = #xs ->
     (∀ (x : A) (xs' : list A),
         xs = x :: xs' →
         pattern η δ p1 #x
           (λ δ',
-            pattern η δ' p2 #xs' φ (ψ2 xs'))
-          (ψ1 x)) ->
+            pattern η δ' p2 #xs' φ (ζ2 xs'))
+          (ζ1 x)) ->
     pattern η δ (pCons p1 p2) v φ
-      (xs = [] \/ (exists x xs', xs = x :: xs' /\ (ψ1 x \/ ψ2 xs'))).
+      (xs = [] \/ (exists x xs', xs = x :: xs' /\ (ζ1 x \/ ζ2 xs'))).
   Proof.
     intros; subst.
-    destruct xs; eapply pattern_exn_mono.
+    destruct xs; eapply pattern_mono_exn.
     { by apply pat_PData_neq. }
     { tauto. }
     { eapply pat_PData_eq; pats. }
@@ -635,54 +622,56 @@ Section pattern_rules.
     | _ => True
     end.
 
-  Lemma cpat_CExc_abst η δ p o φ ψ :
-    (forall e, o = O3Throw e -> pattern η δ p e φ ψ) ->
-    cpattern η δ (CExc p) o φ (is_not_O3Throw o ∨ ψ).
+  Lemma cpat_CExc_abst η δ p o φ ζ :
+    (forall e, o = O3Throw e -> pattern η δ p e φ ζ) ->
+    cpattern η δ (CExc p) o φ (is_not_O3Throw o ∨ ζ).
   Proof.
     intros Hpat.
     unfold cpattern.
     destruct o; simpl.
-    - apply pure_wp_throw. by left.
-    - eapply pure_wp_mono; [ apply Hpat | auto | auto ].
-      reflexivity.
-    - apply pure_wp_throw. by left.
+    - tauto.
+    - eapply pattern_mono_exn.
+      apply Hpat. reflexivity.
+      tauto.
+    - tauto.
   Qed.
 
-  Lemma cpat_CVal_abst η δ p o φ ψ :
-    (forall v, o = O3Ret v -> pattern η δ p v φ ψ) ->
-    cpattern η δ (CVal p) o φ (is_not_O3Ret o ∨ ψ).
+  Lemma cpat_CVal_abst η δ p o φ ζ :
+    (forall v, o = O3Ret v -> pattern η δ p v φ ζ) ->
+    cpattern η δ (CVal p) o φ (is_not_O3Ret o ∨ ζ).
   Proof.
     intros Hpat.
     unfold cpattern.
     destruct o; simpl.
-    - eapply pure_wp_mono; [ apply Hpat | auto | auto ].
-      reflexivity.
-    - apply pure_wp_throw. by left.
-    - apply pure_wp_throw. by left.
+    - eapply pattern_mono_exn. apply Hpat. reflexivity.
+      tauto.
+    - tauto.
+    - tauto.
   Qed.
 
-  Lemma cpat_CEff_abst η δ peff pk o φ ψ1 ψ2 :
+  Lemma cpat_CEff_abst η δ peff pk o φ ζ1 ζ2 :
     (forall eff k,
         o = O3Perform eff k ->
-        pattern η δ peff eff (λ δ, pattern η δ pk (VCont k) φ ψ2) ψ1) ->
-    cpattern η δ (CEff peff pk) o φ (is_not_O3Perform o ∨ ψ1 ∨ ψ2).
+        pattern η δ peff eff (λ δ, pattern η δ pk (VCont k) φ ζ2) ζ1) ->
+    cpattern η δ (CEff peff pk) o φ (is_not_O3Perform o ∨ ζ1 ∨ ζ2).
   Proof.
     intros Hpat.
     unfold cpattern.
     destruct o; simpl.
-    - apply pure_wp_throw. by left.
-    - apply pure_wp_throw. by left.
-    - eapply pure_wp_bind.
-      eapply pure_wp_mono; [ apply Hpat; reflexivity | | auto ].
-      intros δ' Hpat2.
-      eapply pure_wp_mono; [ apply Hpat2 | auto | auto ].
+    - tauto.
+    - tauto.
+    - unfold pattern in Hpat.
+      specialize (Hpat e k eq_refl).
+      destruct (eval_pat η δ peff ); simpl.
+      + eapply pattern_mono_exn; eauto.
+      + tauto.
   Qed.
 
   Lemma cpat_CEff_impossible η δ peff pk (o : outcome2 val exn) φ :
     cpattern η δ (CEff peff pk) o φ True.
   Proof.
     unfold cpattern.
-    destruct o; simpl; by apply pure_wp_throw.
+    by destruct o.
   Qed.
 
 End pattern_rules.
