rocq-osiris/examples/proofs/find.v
@@ -138,7 +138,7 @@ Proof.
       rename xs' into l.
       eapply pure_eval_seq.
       { (* Evaluate [f x]. *)
-        eapply (pure_EApp τ[A]). { pure_path. } { pure_path. apply eq_refl. }
+        eapply (pure_EApp τ[A]). { pure_path. apply Hf. } { pure_path. apply eq_refl. }
         unfold tapp; simpl.
         intros ? <- callsite_f Hcall_f.
         (* Prove that the exceptional postcondition is of the right form. *)
@@ -152,7 +152,8 @@ Proof.
         apply prefix_app; apply prefix_nil. }
       (* Evaluate the second half of the sequence: [iter f l]. *)
       intros Hlprex.
-      eapply (pure_EApp τ[val; list A]). { pure_path. } { pure_path. } { pure_path. apply eq_refl. }
+      eapply (pure_EApp τ[val; list A]).
+      { pure_path. apply IH. } { pure_path. apply eq_refl. } { pure_path. apply eq_refl. }
       simpl; unfold tapp.
       intros ?? <-<- m Hm; unfold listiter_spec in Hm.
       (* Justify the recursive call: the measure has decreased and
@@ -201,7 +202,7 @@ Proof.
     eapply pure_eval_match'_exn.
     { (* Subgoal: evaluate the scrutinee [List.iter _ _]. *)
       eapply (pure_EApp τ[val; list A]); last (simpl; unfold tapp; fold eval).
-      { (* Find iter in the environment. *) pure_path. }
+      { (* Find iter in the environment. *) pure_path. apply Hiter. }
       2:{ (* find [l] in the environment. *) pure_path; apply eq_refl. }
       { (* Evaluate the lambda expression we pass to [iter]:
            it is a function with
@@ -215,7 +216,7 @@ Proof.
           eapply pure_eval_ifthen.
           { (* Subgoal: evaluate the conditional [pred x]. *)
             eapply (pure_EApp τ[A]);
-              [ pure_path | pure_path; apply eq_refl | simpl; unfold tapp ].
+              [ pure_path; apply Hpred | pure_path; apply eq_refl | simpl; unfold tapp ].
             (* We now connect the specs of [pred] and the lambda.
                They have the same success postcondition, so we only need
                to exploit the fact that [pred] cannot fail. *)
@@ -227,7 +228,7 @@ Proof.
             (* Evaluate the constructor [Found x]. *)
             simpl_eval.
             apply pure_wp_Par_vals_right.
-            eapply pure_wp_ret. eapply pure_wp_widen. eapply pure_wp_ret.
+            eapply pure_wp_ret. eapply pure_wp_ret.
             simpl. pure_ret.
             (* Prove the failure postcondition of the lambda.
                That is to say, that [φ] holds for some [x ∈ xs]. *)
