rocq-osiris/theories/program_logic/pure/binding_rules.v
@@ -10,45 +10,45 @@ From osiris.program_logic.pure Require Import wp judgements pattern_rules.
 Definition bindings η bs (φ : env -> Prop) (ψ : exn -> Prop) :=
   pure_wp (eval_bindings η bs) φ ψ.
 
-Lemma pure_wp_irrefutably_extend η δ p v φ ψ :
-  pure_wp (eval_pat η δ p v) φ ⊥ →
-  pure_wp (irrefutably_extend η δ p v) φ ψ.
-Proof.
-  intros H.
-  apply pure_wp_try, (pure_wp_mono _ H);
-    firstorder eauto with pure.
-Qed.
-
 (* -------------------------------------------------------------------------- *)
 
 (* Syntax-directed reasoning rules for the auxiliary judgement [bindings]. *)
 
 Lemma bindings_cons_unary `{Encode A} η p e bs φ :
-  pure (eval η e) (λ a : A, bindings η bs (λ η', pattern η η' p #a φ False) ⊥) ⊥ ->
+  pure (eval η e)
+    (λ a : A,
+       pattern η [] p #a
+         (λ δ1, bindings η bs (λ δ2, φ (δ1 ++ δ2)) ⊥) False) ⊥ ->
   bindings η (Binding p e :: bs) φ ⊥.
 Proof.
   unfold bindings. simpl. intros He.
   simpl_eval_bindings.
   apply pure_wp_Par_vals_left.
+  apply pure_wp_bind.
   apply (pure_wp_mono_ret _ He). intros v (a & -> & Ha).
-  apply (pure_wp_mono_ret _ Ha). intros η' Hη'.
-  eapply pure_wp_widen, pure_wp_try_conseq. eauto.
-  intros. by apply pure_wp_ret. intros _ [].
+  apply pure_wp_widen_pat. unfold continue; simpl.
+  eapply pattern_env_mono. apply Ha. intros δ Hδ.
+  apply (pure_wp_mono_ret _ Hδ). intros η' Hη'.
+  apply pure_wp_ret. apply Hη'.
 Qed.
 
-Lemma bindings_cons `{Encode A} η p e bs (φ1 : A -> Prop) φ2 φ ψ :
+Lemma bindings_cons `{Encode A} η p e bs (φ1 : A -> Prop) φ P Q ψ :
   pure (eval η e) φ1 ψ ->
-  bindings η bs φ2 ψ ->
-  (∀ (a : A) (η' : env), φ1 a -> φ2 η' -> pattern η η' p #a φ False) ->
+  (∀ (a : A), φ1 a -> pattern η [] p #a P False) ->
+  bindings η bs Q ψ ->
+  (∀ η δ, P η → Q δ → φ (η ++ δ)) →
   bindings η (Binding p e :: bs) φ ψ.
 Proof.
-  intros He Hbs Hp.
+  intros He Hp Hbs Hcov.
   unfold bindings.
   simpl_eval_bindings.
   eapply pure_wp_Par_conseq; eauto.
-  - intros _ η' (a & -> & Ha) Hη'.
-    eapply pure_wp_bind, pure_wp_ret, pure_wp_widen, pure_wp_irrefutably_extend. apply Hp; eauto.
-  - intros. eapply pure_wp_bind, pure_wp_throw. tauto.
+  - apply pure_wp_bind.
+    apply (pure_wp_mono_ret _ He). intros ? (? & -> & Hφ1).
+    apply pure_wp_widen_pat, Hp; auto.
+  - intros. unfold continue; simpl.
+    apply pure_wp_ret. auto.
+  - intros exc Hexc. apply pure_wp_throw. tauto.
 Qed.
 
 Lemma bindings_nil η (φ : env -> Prop) ψ :
@@ -68,21 +68,22 @@ Lemma bindings_var `{Encode A} η v e bs (φ : A -> Prop) φ' ψ :
 Proof.
   intros.
   eapply bindings_cons; eauto.
-  intros; unfold pattern. simpl_eval_pat.
-  apply pure_wp_ret; eauto.
+  intros; unfold pattern.
+  eapply (pat_PVar _ _ _ _ (λ η, ∃ a, η = [(v,#a)] ∧ φ a)). eauto.
+  intros ?? (a & -> & Hφ) Hφ'. eauto.
 Qed.
 
-Lemma bindings_pair `{Encode A, Encode B} η p1 p2 e bs φ φ'
-  (φ1 : A -> Prop) (φ2 : B -> Prop) ψ :
+Lemma bindings_pair `{Encode A, Encode B} η p1 p2 e bs φ
+  (φ1 : A -> Prop) (φ2 : B -> Prop) P Q ψ :
   pure (eval η e) (λ '(a, b), φ1 a /\ φ2 b) ψ ->
-  bindings η bs φ' ψ ->
-  (∀ a b η', φ1 a -> φ2 b -> φ' η' -> pattern η η' (PPair p1 p2) #(a, b) φ False) ->
+  (∀ a b η', φ1 a -> φ2 b -> pattern η η' (PPair p1 p2) #(a, b) P False) ->
+  bindings η bs Q ψ ->
+  (∀ η δ, P η → Q δ → φ (η ++ δ)) →
   bindings η (Binding (PPair p1 p2) e :: bs) φ ψ.
 Proof.
-  intros Hpure Hbs Hpat.
+  intros Hpure Hbs Hpat Hcov.
   eapply bindings_cons; eauto.
-  intros [a b] η' [Hψ1 Hψ2] Hη'.
-  auto.
+  intros [a b] [Hψ1 Hψ2]. apply Hbs; auto.
 Qed.
 
 
@@ -94,32 +95,46 @@ Section eval_pat_app.
   Local Ltac rew := repeat (unfold orelse, try, glue2, continue || rewrite ?bind_as_try, ?try2_try2; simpl).
   Local Ltac ext x := let o := fresh "o" in f_equal; extensionality o; destruct o as [ x | ]; auto.
 
-  Lemma eval_pat_app p v η δ : eval_pat η δ p v = 'δ' ← eval_pat η [] p v; ret (δ' ++ δ).
+  Local Open Scope stdpp.
+
+  Lemma eval_pat_app p v η δ :
+    eval_pat η δ p v = δ' ← eval_pat η [] p v; Some (δ' ++ δ).
   Proof.
     revert p v δ.
     apply (pat_ind
-             (λ p, ∀ v δ, eval_pat η δ p v = bind (eval_pat η [] p v) (λ δ', ret (δ' ++ δ)))
-             (λ ps, ∀ vs δ, eval_pats η δ ps vs = bind (eval_pats η [] ps vs) (λ δ', ret (δ' ++ δ)))
-             (λ fps, ∀ vs δ, pre_eval_fpats eval_pat η δ fps vs = bind (pre_eval_fpats eval_pat η [] fps vs) (λ δ', ret (δ' ++ δ)))
+             (λ p, ∀ v δ, eval_pat η δ p v = mbind (λ δ', Some (δ' ++ δ)) (eval_pat η [] p v))
+             (λ ps, ∀ vs δ, eval_pats η δ ps vs = mbind (λ δ', Some (δ' ++ δ)) (eval_pats η [] ps vs) )
+             (λ fps, ∀ vs δ, pre_eval_fpats eval_pat η δ fps vs = mbind (λ δ', Some (δ' ++ δ)) (pre_eval_fpats eval_pat η [] fps vs))
           ); intros ? ?; intros; simpl_eval_pat || simpl_eval_pats || idtac; simpl; auto.
-    - rewrite IHp. rewrite !bind_bind. reflexivity.
-    - rewrite IHp1, IHp2. rew. ext δ'.
+    - rewrite IHp. destruct (eval_pat η [] p v0); auto.
+    - rewrite IHp1, IHp2. destruct (eval_pat η [] p1 v); simpl.
+      + rewrite !union_Some_l. reflexivity.
+      + rewrite !union_None_l. reflexivity.
     - destruct v; auto.
     - destruct v; auto. destruct (_ =? _)%string; auto.
-    - destruct v; auto. rewrite IHps. rew. ext l'. destruct (locations.eqb _ _); auto.
+    - destruct v; auto. rewrite IHps.
+      destruct (lookup_path η π); simpl; auto.
+      destruct (val_as_loc_opt v0); simpl; auto.
+      destruct (locations.eqb _ _); auto.
     - destruct v; auto.
     - destruct v; auto. destruct (int.eq _ _); auto.
     - destruct v; auto. destruct (_ =? _)%char; auto.
     - destruct v; auto. destruct (_ =? _)%string; auto.
     - destruct vs; auto.
-    - destruct vs; auto. rewrite IHp. rew. ext δ1. rew.
-      rewrite (IHps _ δ1), (IHps _ (δ1 ++ _)).
-      rew. ext δ2. rewrite app_assoc. auto.
-    - rew. ext v.
-      rewrite IHp. rew. ext δ1.
-      rewrite IHfps. rew.
-      rewrite (IHfps _ (δ1 ++ _)). rew.
-      ext δ2. rewrite app_assoc. auto.
+    - destruct vs; auto. rewrite IHp.
+      destruct (eval_pat η [] p v); simpl; last reflexivity.
+      rewrite !bind_with_Some.
+      rewrite (IHps _ (e ++ δ)).
+      rewrite (IHps _ e).
+      destruct (eval_pats η [] ps vs); simpl; auto.
+      by rewrite app_assoc.
+    - destruct (lookup_name vs f); simpl; auto.
+      rewrite IHp.
+      destruct (eval_pat η [] p v); simpl; auto.
+      rewrite IHfps.
+      rewrite (IHfps _ e).
+      destruct (pre_eval_fpats eval_pat η [] fps vs); simpl; auto.
+      by rewrite app_assoc.
   Qed.
 End eval_pat_app.
 
@@ -127,9 +142,8 @@ Lemma pattern_app η δ p v φ ψ :
   pattern η δ p v φ ψ ↔ pattern η [] p v (λ δ', φ (δ' ++ δ)) ψ.
 Proof.
   unfold pattern.
-  rewrite eval_pat_app, <-pure_wp_reversible_bind.
-  apply pure_wp_ret_equiv; intros δ'.
-  by rewrite <-pure_wp_reversible_ret.
+  rewrite eval_pat_app.
+  destruct (eval_pat η [] p v); auto.
 Qed.
 
 Definition binding `{Encode A} η p e φ ψ :=
@@ -143,10 +157,7 @@ Lemma binding_bindings_conseq `{Encode A} η p e bs (φ1 φ2 φ : env → Prop) 
 Proof.
   intros He Hbs Hp.
   eapply bindings_cons; eauto.
-  intros a η' Hpa Hη'.
-  apply pattern_app.
-  apply (pure_wp_mono_ret _ Hpa).
-  eauto.
+  intros a Hpa. apply Hpa.
 Qed.
 
 (* May be easier to use but assumes [e] cannot raise exceptions *)
@@ -158,13 +169,13 @@ Proof.
   unfold bindings.
   simpl_eval_bindings.
   apply pure_wp_Par_val_left.
-  apply (pure_wp_mono_ret _ He). intros v (a & -> & Hpa).
-  apply pure_wp_invert_order in Hpa.
-  apply (pure_wp_mono _ Hpa). 2: now apply pure_wp_throw.
-  intros η' Hη'. unfold continue. simpl.
-  eapply pure_wp_widen, pure_wp_irrefutably_extend.
-  rewrite eval_pat_app.
-  apply pure_wp_bind.
-  apply (pure_wp_mono_ret _ Hη').
-  intros. by apply pure_wp_ret.
+  eapply pure_wp_bind_conseq; first apply He.
+  intros v (a & -> & Hpa).
+  apply pure_wp_widen_pat.
+  unfold continue, discontinue; simpl.
+  eapply pattern_env_mono; first apply Hpa.
+  intros δ Hbindings.
+  eapply pure_wp_mono; first apply Hbindings.
+  - intros ? Hφ. apply pure_wp_ret; auto.
+  - intros exc Hexc. apply pure_wp_throw; auto.
 Qed.
