rocq-osiris/theories/program_logic/pure/completeness.v
@@ -14,7 +14,9 @@ Lemma reversible_pat_POr_unary η δ p1 p2 v φ ψ :
   pattern η δ (POr p1 p2) v φ ψ.
 Proof.
   unfold pattern. simpl_eval_pat.
-  apply pure_wp_reversible_orelse.
+  destruct (eval_pat η δ p1 v).
+  - by rewrite union_Some_l.
+  - by rewrite union_None_l.
 Qed.
 
 Lemma reversible_pat_POr η δ p1 p2 v φ ψ :
@@ -23,7 +25,7 @@ Lemma reversible_pat_POr η δ p1 p2 v φ ψ :
   pattern η δ (POr p1 p2) v φ ψ.
 Proof.
   rewrite <-reversible_pat_POr_unary.
-  firstorder eauto using pattern_exn_mono.
+  firstorder eauto using pattern_mono_exn.
 Qed.
 
 Lemma reversible_pat_POr_2 η δ p1 p2 v φ (ψ : Prop) :
@@ -35,7 +37,7 @@ Lemma reversible_pat_POr_2 η δ p1 p2 v φ (ψ : Prop) :
   pattern η δ (POr p1 p2) v φ ψ.
 Proof.
   rewrite <-reversible_pat_POr.
-  firstorder eauto using pattern_exn_mono.
+  firstorder eauto using pattern_mono_exn.
 Qed.
 
 
@@ -47,9 +49,7 @@ Lemma reversible_pat_PData_nil η δ c c' (φ : env → Prop) (ψ : Prop) :
   pattern η δ (PData c nil) (VData c' nil) φ (ψ ∨ c ≠ c').
 Proof.
   unfold pattern; intros. simpl_eval_pat.
-  destruct_string_eqb.
-  rewrite <-pure_wp_reversible_ret. tauto.
-  rewrite <-pure_wp_reversible_throw. tauto.
+  destruct_string_eqb; tauto.
 Qed.
 
 Lemma reversible_pat_PData_or η δ c c' ps vs φ ψ :
@@ -59,72 +59,74 @@ Lemma reversible_pat_PData_or η δ c c' ps vs φ ψ :
 Proof.
   unfold pattern; intros. simpl_eval_pat.
   destruct_string_eqb.
-  - assert (ψ ↔ (ψ ∨ c ≠ c')) by tauto.
-    unfold patterns.
-    firstorder eauto using pure_wp_mono_throw.
-    eapply pure_wp_mono_throw. apply H2. tauto.
-  - rewrite <-pure_wp_reversible_throw. tauto.
+  - unfold patterns.
+    destruct (eval_pats η δ ps vs); tauto.
+  - tauto.
 Qed.
 
 
 (** [PXData], assuming the path lookup is safe *)
 
 Lemma reversible_pat_PXData η δ π ps l l' vs φ ψ :
-  lookup_path η π = ret (VLoc l') →
+  lookup_path η π = Some #l' →
   (l = l' → patterns η δ ps vs φ ψ)
   <->
   pattern η δ (PXData π ps) (VXData l vs) φ (ψ ∨ l ≠ l').
 Proof.
-  unfold pattern. simpl_eval_pat. intros ->.
-  change (as_loc (widen (ret (VLoc l')))) with (@ret _ unit l'). rewrite bind_ret.
+  unfold pattern. simpl_eval_pat. intros ->; simpl.
   destruct (eqb_spec l l').
   - unfold patterns.
-    assert ((ψ ∨ l ≠ l') → ψ) by tauto.
-    firstorder eauto using pure_wp_mono_throw.
-    eapply pure_wp_mono_throw. eassumption. tauto.
-  - rewrite <-pure_wp_reversible_throw. tauto.
+    destruct (eval_pats η δ ps vs); tauto.
+  - tauto.
 Qed.
 
 
 
 (** [PXData] but making no such assumption *)
 
-Lemma lookup_name_cases η x : (∃ v, lookup_name η x = ret v) ∨ lookup_name η x = crash (String.app "missing_variable_or_field: " x).
+Lemma lookup_name_cases η x : (∃ v, lookup_name η x = Some v) ∨ lookup_name η x = None.
 Proof.
   induction η as [ | (y, v) η ]. eauto.
   simpl. destruct (x =? y)%string;eauto.
 Qed.
 
-Lemma lookup_path_cases η π : (∃ v, lookup_path η π = ret v) ∨ lookup_path η π = Crash.
+Lemma lookup_path_cases η π : (∃ v, lookup_path η π = Some v) ∨ lookup_path η π = None.
 Proof.
   revert η; induction π as [ | x π ]; intros η. eauto. simpl.
   destruct (lookup_name_cases η x) as [(v, ->) | ->]; simpl.
   - destruct π; eauto.
-    destruct v; eauto. simpl val_as_struct.
-    rewrite bind_ret.
-    destruct (IHπ xvs) as [(v & ->) | ?]; eauto.
+    destruct v; eauto. simpl val_as_struct_opt.
+    destruct (IHπ xvs) as [(v & Hlookup) | ?]; eauto.
   - destruct π; eauto.
 Qed.
 
 Lemma reversible_pat_PXData_general η δ π ps l vs φ (ψ : Prop) :
   (∃ l',
-      lookup_path η π = ret (VLoc l') ∧
+      (lookup_path η π = Some #l') ∧
       (l = l' → patterns η δ ps vs φ ψ) ∧
-      (l ≠ l' → ψ))
+      (l ≠ l' → ψ)) ∨
+  ((∀ (l' : loc), lookup_path η π ≠ Some #l') ∧ ψ)
   <->
   pattern η δ (PXData π ps) (VXData l vs) φ ψ.
 Proof.
   split.
   - firstorder.
-    eapply pattern_exn_mono.
-    + apply reversible_pat_PXData; eauto.
-    + tauto.
+    + eapply pattern_mono_exn.
+      apply reversible_pat_PXData; eauto.
+      tauto.
+    + unfold pattern. simpl_eval_pat.
+      destruct (lookup_path η π); simpl; last tauto.
+      destruct (val_as_loc_opt v) eqn:Heq.
+      * destruct v; try discriminate Heq.
+        by specialize (H l1).
+      * assumption.
   - unfold pattern. simpl_eval_pat.
-    destruct (lookup_path_cases η π) as [[v ->] | ->]. 2: intros []%invert_pure_wp_crash.
-    assert (widen (ret v) = ret v) as -> by reflexivity.
-    destruct v; try intros []%invert_pure_wp_crash.
-    unfold as_loc; simpl. rewrite bind_ret.
-    destruct (eqb_spec l l0) as [E | N].
+    destruct (lookup_path_cases η π) as [[v ->] | ->]; simpl.
+    + intros Hv; destruct v; try by (right; eauto).
+      left. eexists; split; first reflexivity.
+      simpl in Hv.
+      destruct (eqb_spec l l0) as [E | N].
+      * firstorder.
+      * tauto.
     + firstorder.
-    + intros H%invert_pure_wp_throw; firstorder.
 Qed.
